module part1.Relations where

import Relation.Binary.PropositionalEquality as Eq
open Eq using (_≡_; refl; cong)
open import Data.Nat using (ℕ; zero; suc; _+_; _*_)
open import Data.Nat.Properties using (+-comm; *-comm; +-identityʳ)

data _≤_ : ℕ → ℕ → Set where

  z≤n : ∀ {n : ℕ}
      --------
    → zero ≤ n

  s≤s : ∀ {m n : ℕ}
    → m ≤ n
      -------------
    → suc m ≤ suc n

_ : 2 ≤ 4
_ = s≤s (s≤s z≤n)

-- Give an example of a preorder that is not a partial order.

-- a loves b , b loves a however a != b

-- Give an example of a partial order that is not a total order.

-- um fits inside eg. https://eli.thegreenplace.net/2018/partial-and-total-orders/

-- The above proof omits cases where one argument is z≤n and one argument is s≤s. Why is it ok to omit them?

-- s≤s says both must be suc n however z≤n says one is zero, so the case is not feasible.

≤-refl : ∀ {n : ℕ}
    -----
  → n ≤ n
≤-refl {zero} = z≤n
≤-refl {suc n} = s≤s (≤-refl {n})

≤-trans : ∀ {m n p : ℕ}
    -----
    → m ≤ n
    → n ≤ p
    → m ≤ p
≤-trans z≤n _ = z≤n
≤-trans (s≤s (m≤n)) (s≤s (n≤p)) = s≤s (≤-trans m≤n n≤p)

≤-anti-sym : ∀ {m n : ℕ}
    -----
    → m ≤ n
    → n ≤ m
    → m ≡ n
≤-anti-sym z≤n z≤n = refl
≤-anti-sym (s≤s (m≤n)) (s≤s (n≤m)) = cong suc (≤-anti-sym m≤n n≤m)

data Total (m n : ℕ) : Set where

  forward :
      m ≤ n
      ---------
    → Total m n

  flipped :
      n ≤ m
      ---------
    → Total m n

≤-total : ∀ (m n : ℕ) → Total m n
≤-total zero n       = forward z≤n
≤-total (suc m) zero = flipped z≤n
≤-total (suc m) (suc n) with ≤-total m n
...             | forward m≤n = forward (s≤s m≤n)
...             | flipped n≤m = flipped (s≤s n≤m)

-- ∀ {m n p q : ℕ} → m ≤ n → p ≤ q → m + p ≤ n + q

+-monoʳ-≤ : ∀ (n p q : ℕ)
  → p ≤ q
    -------------
  → (n + p) ≤ (n + q)
+-monoʳ-≤ zero    p q p≤q  =  p≤q
+-monoʳ-≤ (suc n) p q p≤q  =  s≤s (+-monoʳ-≤ n p q p≤q)

+-monoˡ-≤ : ∀ (m n p : ℕ)
  → m ≤ n
    -------------
  → (m + p) ≤ (n + p)
+-monoˡ-≤ m n p m≤n rewrite +-comm m p | +-comm n p  = +-monoʳ-≤ p m n m≤n

+-mono-≤ : ∀ (m n p q : ℕ)
  → m ≤ n
  → p ≤ q
    -------------
  → (m + p) ≤ (n + q)
+-mono-≤ m n p q m≤n p≤q = ≤-trans (+-monoˡ-≤ m n p m≤n) (+-monoʳ-≤ n p q p≤q)

*-monoʳ-≤ : ∀ (n p q : ℕ)
  → p ≤ q
    -------------
  → (n * p) ≤ (n * q)
*-monoʳ-≤ zero    p q p≤q  = z≤n
*-monoʳ-≤ (suc n) p q p≤q  = +-mono-≤ p q (n * p) (n * q) p≤q (*-monoʳ-≤ n p q p≤q)

  -- p ≤ q → (suc n * p) ≤ (suc n * q)
  -- p ≤ q → (p + n * p) ≤ (q + n * q)

*-monoˡ-≤ : ∀ (m n p : ℕ)
  → m ≤ n
    -------------
  → (m * p) ≤ (n * p)
*-monoˡ-≤ m n p m≤n rewrite *-comm m p | *-comm n p  = *-monoʳ-≤ p m n m≤n

*-mono-≤ : ∀ (m n p q : ℕ)
  → m ≤ n
  → p ≤ q
    -------------
  → (m * p) ≤ (n * q)
*-mono-≤ m n p q m≤n p≤q = ≤-trans (*-monoˡ-≤ m n p m≤n) (*-monoʳ-≤ n p q p≤q)
